ocaml/fstar-lib/generated/FStar_Parser_AST_Util.ml
@@ -359,6 +359,8 @@ and (eq_term' :
               (eq_binder b1 b3))
              && (eq_binder b2 b4))
             && (eq_term t4 t8)
+      | (FStar_Parser_AST.DesugaredBlob uu___, FStar_Parser_AST.DesugaredBlob
+         uu___1) -> false
       | uu___ -> false
 and (eq_calc_step :
   FStar_Parser_AST.calc_step -> FStar_Parser_AST.calc_step -> Prims.bool) =
@@ -1110,3 +1112,60 @@ let (register_extension_parser : Prims.string -> extension_parser -> unit) =
 let (lookup_extension_parser :
   Prims.string -> extension_parser FStar_Pervasives_Native.option) =
   fun ext -> FStar_Compiler_Util.smap_try_find extension_parser_table ext
+type extension_lang_parser =
+  {
+  parse_decls:
+    Prims.string ->
+      FStar_Compiler_Range_Type.range ->
+        (error_message, FStar_Parser_AST.decl Prims.list)
+          FStar_Pervasives.either
+    }
+let (__proj__Mkextension_lang_parser__item__parse_decls :
+  extension_lang_parser ->
+    Prims.string ->
+      FStar_Compiler_Range_Type.range ->
+        (error_message, FStar_Parser_AST.decl Prims.list)
+          FStar_Pervasives.either)
+  = fun projectee -> match projectee with | { parse_decls;_} -> parse_decls
+let (extension_lang_parser_table :
+  extension_lang_parser FStar_Compiler_Util.smap) =
+  FStar_Compiler_Util.smap_create (Prims.of_int (20))
+let (register_extension_lang_parser :
+  Prims.string -> extension_lang_parser -> unit) =
+  fun ext ->
+    fun parser ->
+      FStar_Compiler_Util.smap_add extension_lang_parser_table ext parser
+let (lookup_extension_lang_parser :
+  Prims.string -> extension_lang_parser FStar_Pervasives_Native.option) =
+  fun ext ->
+    FStar_Compiler_Util.smap_try_find extension_lang_parser_table ext
+let (parse_extension_lang :
+  Prims.string ->
+    Prims.string ->
+      FStar_Compiler_Range_Type.range -> FStar_Parser_AST.decl Prims.list)
+  =
+  fun lang_name ->
+    fun raw_text ->
+      fun raw_text_pos ->
+        let extension_parser1 = lookup_extension_lang_parser lang_name in
+        match extension_parser1 with
+        | FStar_Pervasives_Native.None ->
+            let uu___ =
+              let uu___1 =
+                FStar_Compiler_Util.format1 "Unknown language extension %s"
+                  lang_name in
+              (FStar_Errors_Codes.Fatal_SyntaxError, uu___1) in
+            FStar_Errors.raise_error uu___ raw_text_pos
+        | FStar_Pervasives_Native.Some parser ->
+            let uu___ = parser.parse_decls raw_text raw_text_pos in
+            (match uu___ with
+             | FStar_Pervasives.Inl error ->
+                 FStar_Errors.raise_error
+                   (FStar_Errors_Codes.Fatal_SyntaxError, (error.message))
+                   error.range
+             | FStar_Pervasives.Inr ds ->
+                 let uu___1 =
+                   FStar_Parser_AST.mk_decl
+                     (FStar_Parser_AST.UseLangDecls lang_name) raw_text_pos
+                     [] in
+                 uu___1 :: ds)
