ocaml/fstar-lib/generated/FStar_Parser_Driver.ml
@@ -43,6 +43,37 @@ let (parse_fragment : FStar_Parser_ParseIt.input_frag -> fragment) =
     | FStar_Parser_ParseIt.Term uu___1 ->
         FStar_Compiler_Effect.failwith
           "Impossible: parsing a Toplevel always results in an ASTFragment"
+let (maybe_dump_module : FStar_Parser_AST.modul -> unit) =
+  fun m ->
+    match m with
+    | FStar_Parser_AST.Module (l, ds) ->
+        let uu___ =
+          let uu___1 = FStar_Ident.string_of_lid l in
+          FStar_Options.dump_module uu___1 in
+        if uu___
+        then
+          let uu___1 = FStar_Ident.string_of_lid l in
+          let uu___2 =
+            let uu___3 =
+              FStar_Compiler_List.map
+                (FStar_Class_Show.show FStar_Parser_AST.showable_decl) ds in
+            FStar_Compiler_String.concat "\n" uu___3 in
+          FStar_Compiler_Util.print2 "Parsed module %s\n%s\n" uu___1 uu___2
+        else ()
+    | FStar_Parser_AST.Interface (l, ds, uu___) ->
+        let uu___1 =
+          let uu___2 = FStar_Ident.string_of_lid l in
+          FStar_Options.dump_module uu___2 in
+        if uu___1
+        then
+          let uu___2 = FStar_Ident.string_of_lid l in
+          let uu___3 =
+            let uu___4 =
+              FStar_Compiler_List.map
+                (FStar_Class_Show.show FStar_Parser_AST.showable_decl) ds in
+            FStar_Compiler_String.concat "\n" uu___4 in
+          FStar_Compiler_Util.print2 "Parsed module %s\n%s\n" uu___2 uu___3
+        else ()
 let (parse_file :
   Prims.string ->
     (FStar_Parser_AST.file * (Prims.string * FStar_Compiler_Range_Type.range)
@@ -52,7 +83,7 @@ let (parse_file :
     let uu___ = FStar_Parser_ParseIt.parse (FStar_Parser_ParseIt.Filename fn) in
     match uu___ with
     | FStar_Parser_ParseIt.ASTFragment (FStar_Pervasives.Inl ast, comments)
-        -> (ast, comments)
+        -> (maybe_dump_module ast; (ast, comments))
     | FStar_Parser_ParseIt.ASTFragment (FStar_Pervasives.Inr uu___1, uu___2)
         ->
         let msg = FStar_Compiler_Util.format1 "%s: expected a module\n" fn in
